Added bigStepExpr definition and also smallStepExpr which recursively calls oneSmallStepExpr; Both don't seem to be working properly unfortunately

While.lean
@@ -1,20 +1,63 @@
 import .WhileSyntax
 open whileSyntax
-open whileSyntax.config
+open whileSyntax.configExpr
 open whileSyntax.wExpr
 open whileSyntax.wComm
 open whileSyntax.wBool
 
 namespace semantics
 
-def smallStep : config → config
-| (configE (ident x, state)) := configE (num (state x), state)
+def a := num 1
+def b := num 2
+def c := num 3
+def d := ident("x")
+def f : string → ℕ
+| "x" := 4
+| _   := 0
+def exampleConfig := (configE(a + b + (c * d), f))
+
+
+def oneSmallStepExpr : configExpr → configExpr
 | (configE (num a, state)) := configE (num a, state)
-| (configE (exp1 + exp2, state)) := let (configE (exp1Eval, _)) := smallStep (configE (exp1, state)) in 
-                                      configE (exp1Eval + exp2, state)
-| (exp1 * exp2) := smallStepExpr exp1 * smallStepExpr exp2
+| (configE (ident x, state)) := configE (num (state x), state)
+| (configE (num a + num b, state)) := configE (num (a + b), state)
+| (configE (num a * num b, state)) := configE (num (a * b), state)
+| (configE (num a + exp2, state)) := let (configE (exp2', state')) := oneSmallStepExpr (configE (exp2, state)) in
+                                       configE (num a + exp2', state')
+| (configE (num a * exp2, state)) := let (configE (exp2', state')) := oneSmallStepExpr (configE (exp2, state)) in
+                                       configE (num a * exp2', state')
+| (configE (exp1 + exp2, state)) := let (configE (exp1', state')) := oneSmallStepExpr (configE (exp1, state)) in 
+                                      configE (exp1' + exp2, state')
+| (configE (exp1 * exp2, state)) := let (configE (exp1', state')) := oneSmallStepExpr (configE (exp1, state)) in 
+                                      configE (exp1' * exp2, state')
 
+def smallStepExpr : configExpr → configExpr
+| (configE (num a, state)) := configE (num a, state)
+| a := have sizeof (oneSmallStepExpr a) < sizeof a, from sorry,
+       smallStepExpr $ oneSmallStepExpr a
 
+def bigStepExpr : configExpr → configExpr
+| (configE (num a, state)) := configE (num a, state)
+| (configE (ident x, state)) := configE (num (state x), state)
+| (configE (num a + num b, state)) := configE (num (a + b), state)
+| (configE (num a * num b, state)) := configE (num (a * b), state)
+| (configE (exp1 + exp2, state)) := let (configE (exp1', state')) := bigStepExpr (configE (exp1, state)),
+                                        (configE (exp2', state'')) := bigStepExpr (configE (exp2, state')) in
+                                      configE (exp1' + exp2', state'')
+| (configE (exp1 * exp2, state)) := let (configE (exp1', state')) := bigStepExpr (configE (exp1, state)),
+                                        (configE (exp2', state'')) := bigStepExpr (configE (exp2, state')) in
+                                      configE (exp1' * exp2', state'')
+
+theorem normal_forms (e : configExpr) : (∃ n : ℕ, ∃ f : string → ℕ, smallStepExpr e = configE (num n, f) ) :=
+begin
+admit
+end
+
+def g := let (configE (a, _)) := smallStepExpr (configE (num 7 + num 6, f)) in a
+def h := let (configE (a, _)) := bigStepExpr (configE (num 7 + ident "x", f)) in a
+def i := let (configE (a, _)) := bigStepExpr exampleConfig in a
+
+#reduce h
 
 
 end semantics
